# 2509.01646v1 - Uniformly-S-projective relative to a module and its dual.pdf



## Page 1

UNIFORMLY-S-PROJECTIVE RELATIVE TO A MODULE AND ITS
DUAL
MOHAMMAD ADARBEH (⋆) AND MOHAMMAD SALEH
ABSTRACT. In this article, we introduce the notion of u-S-projective rela-
tive to a module. Let S be a multiplicative subset of a ring R and M an R-
module. An R-module P is said to be u-S-projective relative to M if for any
u-S-epimorphism f : M →N, the induced map HomR(P, f) : HomR(P,M) →
HomR(P,N) is u-S-epimorphism. Dually, we also introduce u-S-injective rela-
tive to a module. Some properties of these notions are discussed. Several char-
acterizations of u-S-semisimple modules in terms of these notions are given.
The notions of u-S-quasi-projective and u-S-quasi-injective modules are also
introduced and some of their properties are discussed.
1. INTRODUCTION
In this paper, all rings are commutative with nonzero identity and all modules
are unitary. A subset S of a ring R is said to be a multiplicative subset of R if
1 ∈S, 0 /∈S, and s1s2 ∈S for all s1,s2 ∈S. Throughout, R denotes a commutative
ring and S a multiplicative subset of R. Let M be an R-module. M is called a
u-S-torsion module if there exists s ∈S such that sM = 0 [7]. Let M,N,L be an
R-modules.
(i) An R-homomorphism f : M →N is called a u-S-monomorphism (u-S-
epimorphism) if Ker(f) (Coker(f)) is a u-S-torsion module [7].
(ii) An R-homomorphism f : M →N is called a u-S-isomorphism if f is both
a u-S-monomorphism and a u-S-epimorphism [7].
(iii) An R-sequence M
f−→N
g−→L is said to be u-S-exact if there exists s ∈S
such that sKer(g) ⊆Im(f) and sIm(f) ⊆Ker(g). A u-S exact sequence
0 →M →N →L →0 is called a short u-S-exact sequence [6].
(iv) A short u-S-exact sequence 0 →M
f−→N
g−→L →0 is said to be u-S-split
(with respect to s) if there is s ∈S and an R-homomorphism f ′ : N →M
such that f ′ f = s1M, where 1M : M →M is the identity map on M [6].
Qi and Kim et al. [4] introduced the notion of u-S-injective modules. They defind
an R-module E to be u-S-injective if the induced sequence
0 →HomR(C,E) →HomR(B,E) →HomR(A,E) →0
2010 Mathematics Subject Classification. 13Cxx, 13C11, 13C12, 16D40, 16D60.
Key words and phrases. u-S-projective relative to a module, u-S-injective relative to a module,
u-S-quasi-projective, u-S-quasi-injective.
(⋆) Corresponding author.
1
arXiv:2509.01646v1  [math.AC]  1 Sep 2025


## Page 2

2
M. ADARBEH AND M. SALEH
is u-S-exact for any u-S-exact sequence 0 →A →B →C →0. Zhang and Qi [6]
introduced the notion of u-S-projective modules as a dual notion of u-S-injective
modules. They defind an R-module P to be u-S-projective if the induced sequence
0 →HomR(P,A) →HomR(P,B) →HomR(P,C) →0
is u-S-exact for any u-S-exact sequence 0 →A →B →C →0. They also in-
troduced the notions of u-S-semisimple modules and u-S-semisimple rings. An
R-module M is said to be u-S-semisimple if any u-S-short exact sequence 0 →
A →M →C →0 is u-S-split. A ring R is said to be u-S-semisimple ring if
any free R-module is u-S-semisimple. Recall that an R-module U is called pro-
jective (injective) relative to a module M if for each epimorphism (monomor-
phism) f : M →K (g : K →M), the induced map HomR(U, f) : HomR(U,M) →
HomR(U,K) (HomR(g,U) : HomR(M,U) →HomR(K,U)) is an epimorphism
[1]. An R-module M is quasi-projective (quasi-injective) if M is projective (in-
jective) relative to M [1]. The ”uniformly” S-versions of projective (injective)
relative to a module and quasi-projective (quasi-injective) modules are given in
this article (see Definitions 2.1 and 3.1).
In Section 2, we first introduce the notion of u-S-projective relative to a mod-
ule. Dually, we introduce u-S-injective relative to a module, then we investigate
some properties of these notions. For example, we show in Theorem 2.3, that
an R-module P is u-S-projective relative to a module M if and only if for any
submodule K of M, (ηK)∗is u-S-epimorphism, where ηK : M →M
K is the natural
map. We prove in Theorems 2.16 and 2.17 that an R-module M is u-S-semisimple
if and only if every R-module is u-S-injective relative to M if and only if every R-
module is u-S-projective relative to M if and only if for every injective R-module
U and f ∈EndR(U), Ker(f) is u-S-injective relative to M if and only if for every
projective R-module U and f ∈EndR(U), Coker(f) is u-S-projective relative to
M.
In Section 3, we introduce u-S-quasi-projective and u-S-quasi-injective mod-
ules, then we discuss some properties of these notions. Every u-S-projective
(u-S-injective) is u-S-quasi-projective (u-S-quasi-injective). However, the con-
verse is not true (see Examples 3.3 and 3.5). We give in Proposition 3.4, a local
characterization of quasi-projective (quasi-injective) modules. Finally, we give in
Theorem 3.11, a characterization of u-S-semisimple rings in terms of u-S-quasi-
injective and u-S-quasi-projective modules.
2. u-S-PROJECTIVE RELATIVE TO A MODULE AND u-S-INJECTIVE RELATIVE
TO A MODULE
We start this section with the following definition:
Definition 2.1. Let S be a multiplicative subset of a ring R and M an R-modules.
(i) An R-module P is said to be u-S-projective relative to M if for any u-S-
epimorphism f : M →N, the map
HomR(P, f) : HomR(P,M) →HomR(P,N)


## Page 3

UNIFORMLY-S-PROJECTIVE RELATIVE TO A MODULE AND ITS DUAL
3
is u-S-epimorphism.
(ii) An R-module E is said to be u-S-injective relative to M if for any u-S-
monomorphism f : K →M, the map
HomR(f,E) : HomR(M,E) →HomR(K,E)
is u-S-epimorphism.
Remark 2.2. Let S be a multiplicative subset of a ring R and P,E an R-modules.
(a) By [6, Proposition 2.9], P is u-S-projective if and only if P is u-S-projective
relative to every R-module M.
(b) By [6, Proposition 2.5], E is u-S-injective if and only if E is u-S-injective
relative to every R-module M.
For an R-module M, an R-homomorphism f : A →B and K a submodule of
M (K ≤M), let f∗(f ∗) denotes the map HomR(M, f) (HomR(f,M)), iK : K →M
denotes the inclusion map, ηK : M →M
K denotes the natural map.
Theorem 2.3. Let S be a multiplicative subset of a ring R and M,P an R-
modules. Then the following are equivalent:
(1) P is u-S-projective relative to M.
(2) for any epimorphism g : M →N, the map
g∗: HomR(P,M) →HomR(P,N)
is u-S-epimorphism.
(3) for any K ≤M, (ηK)∗is u-S-epimorphism.
Proof. (1) ⇒(2): Clear.
(2) ⇒(3): Apply (2) to the epimorphism ηK : M →M
K . (3) ⇒(1): Let f : M →N
be u-S-epimorphism and K = Ker(f). Then g : M
K →N given by g(x + K) =
f(x) for all x ∈M, is u-S-isomorphism and f = gηK, where ηK : M →M
K is the
natural map. By [6, Lemma 2.1], there is a u-S-isomorphism h : N →M
K and
t ∈S such that hg = t1 M
K . So hf = hgηK = tηK. Since h is u-S-monomorphism,
t′Kerh = 0 for some t′ ∈S. Now by (2), (ηK)∗: HomR(P,M) →HomR(P, M
K ) is
u-S-epimorphism. So there is s ∈S such that sHomR(P, M
K ) ⊆Im(ηK)∗. Take α ∈
HomR(P,N). Then hα ∈HomR(P, M
K ). So shα = (ηK)∗(β) = ηKβ for some β ∈
HomR(P,M). Hence tshα = tηKβ = hfβ. It is easy to chick t′tsα = t′ fβ = ft′β.
So t′tsα ∈Im(f∗). Thus f∗is u-S-epimorphism and therefore, (1) holds.
□
The following result is the dual of Theorem 2.4.
Theorem 2.4. Let S be a multiplicative subset of a ring R and E,M an R-
modules. Then the following are equivalent:
(1) E is u-S-injective relative to M.
(2) for any monomorphism f : K →M, the map
f ∗: HomR(M,E) →HomR(K,E)
is u-S-epimorphism.


## Page 4

4
M. ADARBEH AND M. SALEH
(3) for any K ≤M, (iK)∗is u-S-epimorphism.
Corollary 2.5. Let S be a multiplicative subset of a ring R and M,U an R-
modules. If U is projective (injective) relative to M, then U is u-S-projective
(u-S-injective) relative to M.
Lemma 2.6. Let S be a multiplicative subset of a ring R, fi : Ai →Bi, i = 1,··· ,n
be R-homomorphisms and
nL
i=1
fi :
nL
i=1
Ai →
nL
i=1
Bi be the direct sum map of (fi)n
i=1.
Then
nL
i=1
fi is u-S-epimorphism if and only if each fi is u-S-epimorphism.
Proof. Let f =
nL
i=1
fi. Suppose that f is u-S-epimorphism, then s
nL
i=1
Bi ⊆Im(f) =
nL
i=1
Im(fi) for some s ∈S. So sBi ⊆Im(fi) for each i = 1,··· ,n. Hence each fi
is u-S-epimorphism. Conversely, suppose that each fi is u-S-epimorphism. Then
for each i = 1,··· ,n, there is si ∈S such that siBi ⊆Im(fi). Let s = s1 ···sn. Then
sBi ⊆Im(fi) for each i = 1,··· ,n. Hence s
nL
i=1
Bi =
nL
i=1
sBi ⊆
nL
i=1
Im(fi) = Im(f).
Thus f is u-S-epimorphism.
□
Theorem 2.7. Let S be a multiplicative subset of a ring R and M,A1,··· ,An be
R-modules.
(1)
nL
i=1
Ai is u-S-projective relative to M if and only if each Ai is u-S-projective
relative to M.
(2)
nL
i=1
Ai is u-S-injective relative to M if and only if each Ai is u-S-injective
relative to M.
Proof. We prove only part (1) as the other part is a dual of it. Let f : M →N be
a u-S-epimorphism. Then there are natural isomorphisms α and β such that the
following diagram
HomR
  nL
i=1
Ai,M

α

θ
/ HomR
  nL
i=1
Ai,N

β

nL
i=1
HomR
 Ai,M

λ
/
nL
i=1
HomR
 Ai,N

commutes, where θ = HomR
  nL
i=1
Ai, f

and λ =
nL
i=1
HomR(Ai, f) [1]. Hence
HomR
  nL
i=1
Ai, f

is u-S-epimorphism if and only if
nL
i=1
HomR(Ai, f) is u-S-epimorphism
if and only if each HomR(Ai, f) is u-S-epimorphism by Lemma 2.6. Thus (1)
holds.
□


## Page 5

UNIFORMLY-S-PROJECTIVE RELATIVE TO A MODULE AND ITS DUAL
5
Corollary 2.8. Let S be a multiplicative subset of a ring R and A1,··· ,An be
R-modules.
(1)
nL
i=1
Ai is u-S-projective if and only if each Ai is u-S-projective.
(2)
nL
i=1
Ai is u-S-injective if and only if each Ai is u-S-injective.
Proposition 2.9. Let S be a multiplicative subset of a ring R and M an R-module.
Let f : A →B be u-S-isomorphism. Then
(1) A is u-S-projective (u-S-injective) relative to M if and only if B is u-S-
projective (u-S-injective) relative to M.
(2) M is u-S-projective (u-S-injective) relative to A if and only if M is u-S-
projective (u-S-injective) relative to B.
Proof. We prove only the case of relative u-S-projectivity. First, since f : A →B
is a u-S-isomorphism, so by [6, Lemma 2.1], there is a u-S-isomorphism f ′ : B →
A and t ∈S such that f f ′ = t1B and f ′ f = t1A.
(1) Let g : M →N be a u-S-epimorphism. Since A is u-S-projective relative
to M, then the map
HomR(A,g) : HomR(A,M) →HomR(A,N)
is u-S-epimorphism. So sHomR(A,N) ⊆Im
 HomR(A,g)

for some s ∈S.
Take h ∈HomR(B,N). Then hf ∈HomR(A,N), so shf = gg′ for some
g′ ∈HomR(A,M). Thus sth = sth1B = shf f ′ = gg′ f ′ ∈Im
 HomR(B,g)

(since g′ f ′ ∈HomR(B,M)). Hence B is u-S-projective relative to M. The
other direction is similar.
(2) Let g : B →C be u-S-epimorphism. Since f : A →B is u-S-epimorphism,
gf : A →C is u-S-epimorphism. But M is u-S-projective relative to A,
so (gf)∗= g∗f∗is u-S-epimorphism. So sHomR(M,C) ⊆Im(g∗f∗) ⊆
Im(g∗) for some s ∈S. Thus g∗is u-S-epimorphism. Therefore, M is u-S-
projective relative to B. For the converse, if h : A →C is u-S-epimorphism,
then hf ′ : B →C is u-S-epimorphism. So (hf ′)∗= h∗(f ′)∗is u-S-epimorphism
and hence h∗is u-S-epimorphism. Thus M is u-S-projective relative to A.
□
Lemma 2.10. Let S be a multiplicative subset of a ring R. Consider the following
commutative diagram with exact rows:
A
α

f
/ B
β

g
/ C
γ

D
h
/ E
k
/ F
(1) If β is u-S-epimorphism and h,γ are monomorphisms, then α is u-S-
epimorphism.
(2) If α,γ,g are u-S-epimorphisms, then β is u-S-epimorphism.


## Page 6

6
M. ADARBEH AND M. SALEH
(3) If 0 →A
f−→B
g−→C →0 is a u-S-split exact sequence, then HomR(M,g)
is u-S-epimorphism for any R-module M.
Proof.
(1) Since β is u-S-epimorphism, so sE ⊆Im(β) for some s ∈S. Let
d ∈D. Then h(d) ∈E implies sh(d) = β(b) for some b ∈B. So kβ(b) =
skh(d) = 0 but then γg(b) = 0. But γ is a monomorphism, so g(b) = 0
and this implies b ∈Ker(g) = Im(f). So b = f(a) for some a ∈A. Hence
sh(d) = β(b) = β(f(a)) = β f(a) = hα(a). Since h is a monomorphism,
sd = α(a). Thus α is u-S-epimorphism.
(2) Similar to the proof of [4, Lemma 2.11].
(3) By [6, Lemma 2.4], there is s ∈S and g′ : C →B such that gg′ = s1C.
For h ∈HomR(M,C), then sh = s1Ch = sgg′h ∈Im
 HomR(M,g)

. Thus
HomR(M,g) is u-S-epimorphism.
□
Theorem 2.11. Let S be a multiplicative subset of a ring R and M an R-module.
(1) Let A be a submodule of B. If M is u-S-projective relative to B, then M is
u-S-projective relative to both A and B
A.
(2) M is u-S-projective relative to
nL
i=1
Ai if and only if M is u-S-projective
relative to each Ai.
Proof.
(1) Since ηA : B →B
A is an epimorphism and M is u-S-projective rel-
ative to B, then by the first part of Proposition 2.9 (2), we have M is
u-S-projective relative to B
A. Now let K ≤A and consider the commuta-
tive diagram
0

0
/ A
ηK

/ B

/ B
A

/ 0
0
/ A
K

/ B
K

/ B
A

/ 0
0
0
0
with exact rows and columns. Since M is u-S-projective relative to B
and HomR(M,−) is left exact, we have the commutative diagram


## Page 7

UNIFORMLY-S-PROJECTIVE RELATIVE TO A MODULE AND ITS DUAL
7
0

0
/ HomR(M,A)
(ηK)∗

/ HomR(M,B)

/ HomR(M, B
A)

0
/ HomR(M, A
K)
/ HomR(M, B
K)

/ HomR(M, B
A)

0
0
with exact rows and columns. By Lemma 2.10 (1), (ηK)∗is u-S-epimorphism.
Thus, by Theorem 2.3, M is u-S-projective relative to A.
(2) We prove this part only for n = 2. Suppose that M is u-S-projective rela-
tive to A⊕B. Since A⊕B
A
∼= B, then by part (1), M is u-S-projective relative
to both A and B. Conversely, suppose that M is u-S-projective relative to
both A and B. Let K ≤A ⊕B. Then there is an obvious commutative
diagram
0
/ A

/ A⊕B
ηK 
/ B

/ 0
0
/ A+K
K

/ A⊕B
K

/ A⊕B
A+K

/ 0
0
0
0
with exact rows and columns. Since M is u-S-projective relative to both
A and B, then by applying HomR(M,−) to the above diagram, we obtain
the following commutative diagram
0
/ HomR(M,A)

/ HomR(M,A⊕B)
(ηK)∗
/ HomR(M,B)

0
/ HomR(M, A+K
K )

/ HomR(M, A⊕B
K )
/ HomR(M, A⊕B
A+K)

0
0
with exact rows and columns. Since 0 →A →A ⊕B →B →0 splits,
then by Lemma 2.10 (2) and (3), we have (ηK)∗is u-S-epimorphism.
Therefore, by Theorem 2.3, M is u-S-projective relative to A⊕B.
□
Theorem 2.12. Let S be a multiplicative subset of a ring R and M an R-module.


## Page 8

8
M. ADARBEH AND M. SALEH
(1) Let A be a submodule of B. If M is u-S-injective relative to B, then M is
u-S-injective relative to both A and B
A.
(2) M is u-S-injective relative to
nL
i=1
Ai if and only if M is u-S-injective rela-
tive to each Ai.
Proof. Similar to the proof of Theorem 2.11.
□
Corollary 2.13. Let S be a multiplicative subset of a ring R and let 0 →A
f−→B
g−→
C →0 be a u-S-exact sequence. If M is u-S-projective (u-S-injective) relative to
B, then M is u-S-projective (u-S-injective) relative to both A and C.
Proof. Let 0 →A
f−→B
g−→C →0 be a u-S-exact sequence. Then A is u-S-isomorphic
to Im(f) and C is u-S-isomorphic to
B
Ker(g). Since M is u-S-projective (u-S-
injective) relative to B, then by Theorems 2.11 and 2.12, M is u-S-projective
(u-S-injective) relative to Im(f) and also M is u-S-projective (u-S-injective) rel-
ative to
B
Ker(g). Hence by Proposition 2.9 (2), M is u-S-projective (u-S-injective)
relative to both A and C.
□
Proposition 2.14. Let S be a multiplicative subset of a ring R and let 0 →
A →B →C →0 be a u-S-split exact sequence. Then M is u-S-projective (u-
S-injective) relative to B if and only if M is u-S-projective (u-S-injective) relative
to both A and C.
Proof. Since the exact sequence 0 →A →B →C →0 u-S-splits, then by [2,
Lemma 2.8], B is u-S-isomorphic to A⊕C. So if M is u-S-projective (u-S-injective)
relative to both A and C, then by Theorems 2.11 and 2.12, M is u-S-projective
(u-S-injective) relative to A ⊕C and hence by Proposition 2.9 (2), M is u-S-
projective (u-S-injective) relative to B. The other direction follows from Corol-
lary 2.13.
□
Lemma 2.15. Let S be a multiplicative subset of a ring R. A u-S-exact sequence
0 →A
f−→B
g−→C →0 u-S-splits if either A is u-S-injective relative to B or C is
u-S-projective relative to B.
Proof. First, suppose that A is u-S-injective relative to B, then
f ∗: HomR(B,A) →HomR(A,A)
is u-S-epimorphism. So sHomR(A,A) ⊆Im(f ∗) for some s ∈S. So s1A ∈Im(f ∗)
and hence s1A = f ∗(f ′) = f ′ f for some f ′ ∈HomR(B,A). Thus 0 →A
f−→B
g−→
C →0 u-S-splits. Next, suppose that C is u-S-projective relative to B. Then
g∗: HomR(C,B) →HomR(C,C)
is u-S-epimorphism. So tHomR(C,C) ⊆Im(g∗) for some t ∈S. So t1C ∈Im(g∗)
and hence t1C = g∗(g′) = gg′ for some g ∈HomR(C,B). Thus by [6, Lemma
2.4], 0 →A
f−→B
g−→C →0 u-S-splits.
□


## Page 9

UNIFORMLY-S-PROJECTIVE RELATIVE TO A MODULE AND ITS DUAL
9
The last two results of this section give new characterizations of u-S-semisimple
modules.
Theorem 2.16. Let R be a ring and S a multiplicative subset of R. The following
statements about an R-module M are equivalent:
(1) M is u-S-semisimple.
(2) Every R-module is u-S-injective relative to M.
(3) Every R-module is u-S-projective relative to M.
Proof. (1) ⇒(2): Let N be any R-module and f : K →M be a u-S-monomorphism.
Then by (1), 0 →K
f−→M →Coker(f) →0 u-S-splits. So there is an R-homomorphism
f ′ : M →K and s ∈S such that f ′ f = s1K. For any h ∈HomR(K,N), sh = hs1K =
hf ′ f = f ∗(hf ′) and hf ′ ∈HomR(M,N). So f ∗: HomR(M,N) →HomR(K,N) is
u-S-epimorphism. Thus N is u-S-injective relative to M. Since N was an arbitrary
R-module, (2) holds.
(1) ⇒(3): Let N be any R-module and g : M →L be a u-S-epimorphism. Then
by (1), 0 →Ker(g) →M
g−→L →0 u-S-splits. So there is an R-homomorphism
g′ : L →M and s ∈S such that gg′ = s1L. For any h ∈HomR(N,L), sh = s1Lh =
gg′h = g∗(g′h) and g′h ∈HomR(N,M). So g∗: HomR(N,M) →HomR(N,L) is
u-S-epimorphism. Thus N is u-S-projective relative to M. Since N was an arbi-
trary R-module, (3) holds.
(2) ⇒(1): Let 0 →A →M →C →0 be a u-S-exact sequence. Then by (2), A is
u-S-injective relative to M. So by Lemma 2.15, 0 →A →M →C →0 u-S-splits.
Hence M is u-S-semisimple.
(3) ⇒(1): Let 0 →A →M →C →0 be a u-S-exact sequence. Then by (3), C
is u-S-projective relative to M. Hence by Lemma 2.15, 0 →A →M →C →0
u-S-splits. Thus M is u-S-semisimple.
□
For an R-module M, let E(M) denotes the injective envelope of M.
Theorem 2.17. Let R be a ring and S a multiplicative subset of R. The following
statements about an R-module M are equivalent:
(1) M is u-S-semisimple.
(2) For every injective R-module U and f ∈EndR(U), Ker(f) is u-S-injective
relative to M.
(3) For every projective R-module U and f ∈EndR(U), Coker(f) is u-S-
projective relative to M.
Proof. (1) ⇒(2) and (1) ⇒(3) follow from Theorem 2.16.
(2) ⇒(1): Let N be any R-module. We show that N is u-S-injective relative to
M. Consider the injective R-module U = E(N)⊕E
 E(N)
N

. Define f : U →U by
f(x,y) = (0,x+N). Then it is easy to check that f ∈EndR(U) and Ker(f) = N ⊕
E
 E(N)
N

. By (2), Ker(f) is u-S-injective relative to M. So by Theorem 2.7 (2), N
is u-S-injective relative to M. Hence every R-module is u-S-injective relative to


## Page 10

10
M. ADARBEH AND M. SALEH
M and thus by Theorem 2.16, M is u-S-semisimple.
(3) ⇒(1): Let 0 →A α−→M
β−→C →0 be a u-S-exact sequence and K = Ker(β).
Then C is u-S-isomorphic to M
K . Let g : P →M be an epimorphism with P is
projective. Let N = Ker(ηKg), where ηK : M →M
K is the natural map. Then N ≤
P and M
K ∼= P
N. There is an epimorphism h : P′ →N with P′ is projective. Let
U = P ⊕P′, then U is projective. Now define f : U →U by f(x,y) = (h(y),0).
Then f ∈EndR(U) and Im(f) = N ⊕0. Now Coker(f) =
U
Im(f) = P⊕P′
N⊕0 ∼= P
N ⊕P′.
By (3), Coker(f) = P
N ⊕P′ is u-S-projective relative to M. So by Theorem 2.7
(1) and Proposition 2.9 (1), M
K ∼= P
N is u-S-projective relative to M. But C is u-S-
isomorphic to M
K , so again by Proposition 2.9 (1), C is u-S-projective relative to
M. Hence, by Lemma 2.15, 0 →A α−→M
β−→C →0 is u-S-split. Therefore, M is
u-S-semisimple.
□
3. u-S-QUASI-PROJECTIVE AND u-S-QUASI-INJECTIVE MODULES
We begin this section with the following definition:
Definition 3.1. Let R be a ring and S be a multiplicative subset of R. An R-
module M is said to be u-S-quasi-projective (u-S-quasi-injective) if M is u-S-
projective relative to M (u-S-injective relative to M).
Remark 3.2. Let R be a ring and S be a multiplicative subset of R.
(1) By Remark 2.2, every u-S-projective (u-S-injective) R-module is u-S-
quasi-projective (u-S-quasi-injective).
(2) By Corollary 2.5, every quasi-projective (quasi-injective) R-module is u-
S-quasi-projective (u-S-quasi-injective).
The following example gives a u-S-quasi-projective module that is not u-S-
projective.
Example 3.3. Let R = Z and S = N = {1,2,3,···}. If P is the set of all prime
numbers, then L
P Zp is quasi-projective [1] and hence it is u-S-quasi-projective.
But since Ext1
R
 L
P Zp,Z
 ∼= ∏P Ext1
R(Zp,Z) ∼= ∏P Zp is not u-S-torsion, then
by [6, Proposition 2.9], L
P Zp is not u-S-projective.
Let p be a prime ideal of a ring R. Then S = R\p is a multiplicative subset of
R. We say that an R-module M is u-p-quasi-projective (u-p-quasi-injective) if M
is u-S-quasi-projective (u-S-quasi-injective). The following result gives a local
characterization of quasi-projective (quasi-injective) modules.
For a ring R, let Max(R) denotes the set of all maximal ideals of R and
Spec(R) denotes the set of all prime ideals of R.
Proposition 3.4. Let S be a multiplicative subset of a ring R and M an R-module.
Then the following statements are equivalent:
(1) M is quasi-projective (quasi-injective).


## Page 11

UNIFORMLY-S-PROJECTIVE RELATIVE TO A MODULE AND ITS DUAL
11
(2) M is u-p-quasi-projective (u-p-quasi-injective) for every p ∈Spec(R).
(3) M is u-m-quasi-projective (u-m-quasi-injective) for every m ∈Max(R).
Proof. We prove only the case of quasi-projectivity. (1) ⇒(2) and (2) ⇒(3) are
clear. (3) ⇒(1): Let f : M →N be an epimorphism. We show that the map
f∗: HomR(M,M) →HomR(M,N)
is an epimorphism. That is, Coker(f∗) = 0. By (3), for every m ∈Max(R), there
exists sm ∈S such that smCoker(f∗) = 0. But since ⟨{sm | m ∈Max(R)}⟩= R.
So there exist r1,··· ,rn ∈R and m1,··· ,mn ∈Max(R) such that 1 = r1sm1 +···+
rnsmn. Hence we have Coker(f∗) = (r1sm1 +···+rnsmn)Coker(f∗) ⊆r1sm1Coker(f∗)+
···+rnsmnCoker(f∗) = 0. Thus Coker(f∗) = 0. Therefore, M is quasi-projective.
□
The following example provides a u-S-quasi-injective module that is not u-S-
injective.
Example 3.5. Let R = Z and M = Z2. Then M is a simple R-module and hence it
is quasi-injective. But M is not injective R-module, so by [4, proposition 4.8], M
is not u-m-injective for some maximal ideal m of R. However, M is u-m-quasi-
injective.
Proposition 3.6. Let S be a multiplicative subset of a ring R and M an R-
module. If M is u-S-semisimple, then M is both u-S-quasi-injective and u-S-
quasi-projective.
Proof. Let M be a u-S-semisimple module. Then by Theorem 2.16, every R-
module is u-S-injective (u-S-projective) relative to M. In particular, M is u-S-
injective (u-S-projective) relative to M. Thus M is both u-S-quasi-injective and
u-S-quasi-projective.
□
The following example gives a u-S-quasi-injective module that is not quasi-
injective.
Example 3.7. Let R = Z and S = Z\{0}. Then by [6, Example 3.7], Z is a u-S-
semisimple Z-module, so by Proposition 3.6, Z is u-S-quasi-injective Z-module.
However, Z is not a quasi-injective Z-module [3, Example 2.3].
Proposition 3.8. Let S be a multiplicative subset of a ring R. Then
nL
i=1
Ai is u-
S-quasi-projective (u-S-quasi-injective) if and only if Ai is u-S-projective (u-S-
injective) relative to Aj for each i, j = 1,2,··· ,n.
Proof. By Theorems 2.7, 2.11 and 2.12, we have
nL
i=1
Ai is u-S-quasi-projective
(u-S-quasi-injective) if and only if
nL
i=1
Ai is u-S-projective (u-S-injective) relative
to
nL
i=1
Ai if and only if Ai is u-S-projective (u-S-injective) relative to
nL
j=1
Aj for


## Page 12

12
M. ADARBEH AND M. SALEH
each i = 1,2,··· ,n if and only if Ai is u-S-projective (u-S-injective) relative to A j
for each i, j = 1,2,··· ,n.
□
Proposition 3.9. Let S be a multiplicative subset of a ring R and B be a u-S-
quasi-projective R-module. Then an exact sequence 0 →A
f−→B
g−→C →0 u-S-
splits if and only if C is u-S-projective relative to B.
Proof. Let B be a u-S-quasi-projective and let 0 →A
f−→B
g−→C →0 be u-S-
split exact sequence. Then by [2, Lemma 2.8], B is u-S-isomorphic to A⊕C. So
by Proposition 2.9, A ⊕C is u-S-quasi-projective. Hence by Proposition 3.8, C
is u-S-projective relative to both A and C. Thus by Proposition 2.14, C is u-S-
projective relative to B. The converse follows from Lemma 2.15.
□
Proposition 3.10. Let S be a multiplicative subset of a ring R and B be a u-S-
quasi-injective R-module. Then an exact sequence 0 →A
f−→B
g−→C →0 u-S-
splits if and only if A is u-S-injective relative to B.
Proof. The proof is similar to that of Proposition 3.9
□
Lastly, we give a characterization of u-S-semisimple rings in terms of u-S-
quasi-injective and u-S-quasi-projective modules.
Theorem 3.11. Let R be a ring and S a multiplicative subset of R. The following
statements are equivalent:
(1) R is u-S-semisimple.
(2) Every R-module is u-S-quasi-injective
(3) Every R-module is u-S-quasi-projective.
Proof. (1) ⇒(2) and (1) ⇒(3) follow from [6, Theorem 3.5] and the fact that
every u-S-injective (u-S-projective) is u-S-quasi-injective (u-S-quasi-projective).
(2) ⇒(1): Let M be any R-module. Then for any R-module N, M ⊕N is u-
S-quasi-injective. So by Proposition 3.8, N is u-S-injective relative to M. Thus
every R-module is u-S-injective relative to M. Hence by Theorem 2.16, M is
u-S-semisimple. Since M was an arbitrary R-module, so every R-module is u-S-
semisimple. Thus by [6, Theorem 3.5], R is u-S-semisimple.
(3) ⇒(1): Similar to the proof of the implication (2) ⇒(1).
□
REFERENCES
[1] F.W. Anderson and K.R. Fuller, Rings and Categories of Modules (Springer-
Verlag 1974).
[2] H. Kim, N. Mahdou, E. H. Oubouhou and X. Zhang, Uniformly S-projective
modules and uniformly S-projective uniformly S-covers, Kyungpook Math.
J., 64 (2024), 607–618.
[3] V. Kumar, A. J. Gupta, B. M. Pandeya and M. K. Patel, M-C-Pseudo Injec-
tive Modules, East-West J. of Mathematics: Vol. 14, No 1(2012) pp. 67-75.


## Page 13

UNIFORMLY-S-PROJECTIVE RELATIVE TO A MODULE AND ITS DUAL
13
[4] W. Qi, H. Kim, F. G. Wang, M. Z. Chen and W. Zhao, Uniformly S-
Noetherian rings, Quaest. Math., 47(5) (2023), 1019–1038.
[5] F. Wang and H. Kim, Foundations of Commutative Rings and Their Mod-
ules, Algebra and Applications, vol. 22, Springer, Singapore, 2016.
[6] X. L. Zhang and W. Qi, Characterizing S-projective modules and S-
semisimple rings by uniformity, J. Commut. Algebra, 15(1) (2023), 139-
149.
[7] X. L. Zhang, Characterizing S-flat modules and S-von Neumann regular
rings by uniformity, Bull. Korean Math. Soc., 59 (2022), no. 3, 643-657.
DEPARTMENT OF MATHEMATICS, BIRZEIT UNIVERSITY, BIRZEIT, PALESTINE
Email address: madarbeh@birzeit.edu
DEPARTMENT OF MATHEMATICS, BIRZEIT UNIVERSITY, BIRZEIT, PALESTINE
Email address: msaleh@birzeit.edu
